verify/Individual62.v
@@ -161,16 +161,6 @@ Proof.
     reflexivity.
 Qed.
 
-Lemma lpow_mul{A} (a:list A) b n:
-  a^^(b*n) = (a^^n)^^b.
-Proof.
-  induction b.
-  - reflexivity.
-  - cbn.
-    rewrite lpow_add.
-    congruence.
-Qed.
-
 Lemma lpow_shift21e(a:Sym)(b:Stream Sym) n:
   a >> [a;a]^^n *> b = [a;a]^^n *> a >> b.
 Proof.
