verify/LongLoop3x3v1.v
@@ -1,0 +1,389 @@
+From BusyCoq Require Import LongLoop.
+From BusyCoq Require Import Individual33.
+
+Module LongLoop62 := LongLoop BB33.
+Import LongLoop62.
+
+Require Import ZArith.
+Require Import String.
+
+Close Scope N.
+
+Import Eqb.
+
+Lemma find_spec {X Y} {E:Eqb X} (x0:X) ls (y0:Y):
+  List.find (fun '(x,y) => eqb x x0) ls &&& (fun '(x,y) => Some y) = Some y0 ->
+  List.In (x0,y0) ls.
+Proof.
+  intros.
+  unfold if_Some in H.
+  destruct (List.find (fun '(x,_) => eqb x x0)) eqn:E0.
+  2: inverts H.
+  eapply List.find_some in E0.
+  destruct E0 as [I1 I2].
+  destruct p as [x y].
+  destruct (eqb_spec x x0); [|inverts I2].
+  subst.
+  inverts H; trivial.
+Qed.
+
+Lemma f2_spec' tm ls T:
+  List.forallb (fun '(h,w,(a0,a1,h')) =>
+  BoundedConfig.segRLs_c tm ([h] ^^ N.to_nat (2 ^ a0)) ([h'] ^^ N.to_nat (2 ^ a1)) w w T) ls = true ->
+  forall w h a0 a1 h',
+  List.In (h, w, (a0, a1, h')) ls ->
+  segRLs tm ([h] ^^ N.to_nat (2 ^ a0)) ([h'] ^^ N.to_nat (2 ^ a1)) w w.
+Proof.
+  intros.
+  rewrite List.forallb_forall in H.
+  apply H in H0.
+  apply BoundedConfig.segRLs_c_spec in H0.
+  apply H0.
+Qed.
+
+Lemma f1_spec' tm ls T:
+  List.forallb (fun '(h,w,(ws,hs)) => BoundedConfig.segRLs_c tm [h] hs w (List.concat ws) T) ls = true ->
+  forall w h ws hs,
+  List.In (h, w, (ws, hs)) ls ->
+  segRLs tm [h] hs w (List.concat ws).
+Proof.
+  intros.
+  rewrite List.forallb_forall in H.
+  apply H in H0.
+  apply BoundedConfig.segRLs_c_spec in H0.
+  apply H0.
+Qed.
+
+Lemma f0_spec' tm ls T:
+  List.forallb (fun '(h,w,(ws',w')) => BoundedConfig.sideRLs_c tm [h] w ((List.concat ws')++w') T) ls = true ->
+  forall w h w',
+  List.In (h, w, w') ls ->
+  sideRLs tm [h] (w *> 0inf) (to_side w').
+Proof.
+  intros.
+  rewrite List.forallb_forall in H.
+  apply H in H0.
+  destruct w' as [ws' w'].
+  apply BoundedConfig.sideRLs_c_spec in H0.
+  rewrite Str_app_assoc in H0.
+  apply H0.
+Qed.
+
+Ltac stepn n0 :=
+  eapply without_counter with (n:=N.to_nat n0);
+  eapply multistep_c_spec; vm_compute; repeat rewrite <-const_unfold; reflexivity.
+
+
+Module TM1.
+Definition tm := Eval compute in (TM_from_str "1LB2LB1RC_1RA2LB0LB_2RB---0RA").
+Notation "c -->* c'" := (c -[ tm ]->* c') (at level 40).
+Notation "c -->+ c'" := (c -[ tm ]->+ c') (at level 40).
+
+Notation h0 := ((A,<[]),(B,[])).
+Notation h1 := ((C,<[1]),(B,[])).
+Notation h2 := ((B,<[1;2]),(B,[])).
+
+Definition f1 (w:seg)(h:head):option((list seg)*(list head)) :=
+List.find (fun '(x,y) => eqb x (h,w)) (
+((h0,[2;2]),([[2;2]],[h0;h0]))::
+((h0,[2;0;2]),([[2;0;0]],[]))::
+((h0,[2;0;0]),([[2;0;2]],[h0]))::
+((h1,[2;2]),([[2;2]],[h1;h0]))::
+((h1,[2;0;2]),([[2;2];[2;2]],[]))::
+((h1,[2;0;0]),([[2;2];[2;0]],[]))::
+((h0,[2;0]),([],[h2]))::
+((h2,[2;0;0]),([[2;0;0];[0;0]],[]))::
+((h0,[0;0]),([[1;0]],[]))::
+((h0,[1;0]),([[2;0]],[]))::
+((h2,[2;0;2]),([[2;0;0];[0;2]],[]))::
+((h0,[0;2]),([[1;2]],[]))::
+((h0,[1;2]),([[2;2]],[]))::
+((h2,[2;2]),([[2;0;0];[2]],[]))::
+((h0,[2]),([],[h1]))::
+nil) &&& (fun '(x,y) => Some y).
+
+Definition f0 (w:seg)(h:head):option((list seg)*seg) :=
+List.find (fun '(x,y) => eqb x (h,w)) (
+((h0,[1]),([],[2]))::
+((h0,[2]),([[2;0;2]],[1]))::
+nil) &&& (fun '(x,y) => Some y).
+
+Definition f2 (w:seg)(h:head):option(N*N*head) :=
+List.find (fun '(x,y) => eqb x (h,w)) (
+((h0,[2;2]),(0%N,1%N,h0))::
+((h0,[2;0;2]),(1%N,0%N,h0))::
+((h0,[2;0;0]),(1%N,0%N,h0))::
+nil) &&& (fun '(x,y) => Some y).
+
+Definition ws_init:(list seg)*seg := ([[2;2];[2;2];[2;2];[2;2];[2;0;2];[2;0;2];[2;0;2]],[1]).
+
+Definition hs_step:(list head) := [h1]^^30.
+
+
+Lemma nonhalt: ~halts tm c0.
+Proof.
+  eapply decide_nonhalt_spec with
+  (tm:=tm) (f2:=f2) (f1:=f1) (f0:=f0) (hs_step:=hs_step) (ws_init:=ws_init)
+  (lh:=0inf<*<[1]) (pp:=1%nat) (T:=N.to_nat (10^5)).
+  - intros.
+    unfold f2 in H.
+    apply find_spec in H.
+    gen w h a0 a1 h'.
+    apply f2_spec' with (T:=(10^3)).
+    time vm_compute; reflexivity.
+  - intros.
+    unfold f1 in H.
+    apply find_spec in H.
+    gen w h ws hs.
+    apply f1_spec' with (T:=(10^3)).
+    time vm_compute; reflexivity.
+  - intros.
+    unfold f0 in H.
+    apply find_spec in H.
+    gen w h w'.
+    apply f0_spec' with (T:=(10^3)).
+    time vm_compute; reflexivity.
+  - reflexivity.
+  - intro X; inverts X.
+  - apply BoundedConfig.sideRLs_c_spec with (T:=10^4); reflexivity.
+  - stepn 314%N.
+  - native_check_eq.
+Time Qed.
+
+End TM1.
+
+
+Module TM2.
+Definition tm := Eval compute in (TM_from_str "1LB1RC1RC_1RA2LB0LB_2RB---0RA").
+Notation "c -->* c'" := (c -[ tm ]->* c') (at level 40).
+Notation "c -->+ c'" := (c -[ tm ]->+ c') (at level 40).
+
+Notation h0 := ((A,<[]),(B,[])).
+Notation h1 := ((C,<[1]),(B,[])).
+Notation h2 := ((B,<[1;2]),(B,[])).
+
+Definition f1 (w:seg)(h:head):option((list seg)*(list head)) :=
+List.find (fun '(x,y) => eqb x (h,w)) (
+((h0,[2;2]),([[2;2]],[h0;h0]))::
+((h0,[2;0;2]),([[2;0;0]],[]))::
+((h0,[2;0;0]),([[2;0;2]],[h0]))::
+((h1,[2;2]),([[2;2]],[h1;h0]))::
+((h1,[2;0;0]),([[2;2]],[h2]))::
+((h2,[2;0;2]),([[2;0;0];[0;2]],[]))::
+((h0,[0;2]),([[1;2]],[]))::
+((h0,[1;2]),([[2;2]],[h0;h0]))::
+((h2,[2;2]),([[2;0;0];[2]],[]))::
+((h0,[2]),([],[h1]))::
+((h1,[2;0;2]),([[2;2];[2;2]],[h0;h0]))::
+((h2,[2;0;0]),([[2;0;0];[0;0]],[]))::
+((h0,[0;0]),([[1;0]],[]))::
+((h0,[1;0]),([],[h2]))::
+nil) &&& (fun '(x,y) => Some y).
+
+Definition f0 (w:seg)(h:head):option((list seg)*seg) :=
+List.find (fun '(x,y) => eqb x (h,w)) (
+((h0,[1]),([[2;0;2]],[1]))::
+nil) &&& (fun '(x,y) => Some y).
+
+Definition f2 (w:seg)(h:head):option(N*N*head) :=
+List.find (fun '(x,y) => eqb x (h,w)) (
+((h0,[2;2]),(0%N,1%N,h0))::
+((h0,[2;0;2]),(1%N,0%N,h0))::
+((h0,[2;0;0]),(1%N,0%N,h0))::
+nil) &&& (fun '(x,y) => Some y).
+
+Definition ws_init:(list seg)*seg := ([[2;2];[2;2];[2;2];[2;2];[2;2];[2;0;0];[2;0;2];[2;0;2];[2;0;2];[2;0;2]],[1]).
+
+Definition hs_step:(list head) := [h1]^^15.
+
+
+Lemma nonhalt: ~halts tm c0.
+Proof.
+  eapply decide_nonhalt_spec with
+  (tm:=tm) (f2:=f2) (f1:=f1) (f0:=f0) (hs_step:=hs_step) (ws_init:=ws_init)
+  (lh:=0inf<*<[1]) (pp:=4%nat) (T:=N.to_nat (10^5)).
+  - intros.
+    unfold f2 in H.
+    apply find_spec in H.
+    gen w h a0 a1 h'.
+    apply f2_spec' with (T:=(10^3)).
+    time vm_compute; reflexivity.
+  - intros.
+    unfold f1 in H.
+    apply find_spec in H.
+    gen w h ws hs.
+    apply f1_spec' with (T:=(10^3)).
+    time vm_compute; reflexivity.
+  - intros.
+    unfold f0 in H.
+    apply find_spec in H.
+    gen w h w'.
+    apply f0_spec' with (T:=(10^3)).
+    time vm_compute; reflexivity.
+  - reflexivity.
+  - intro X; inverts X.
+  - apply BoundedConfig.sideRLs_c_spec with (T:=10^4); reflexivity.
+  - stepn 593%N.
+  - native_check_eq.
+Time Qed.
+
+End TM2.
+
+
+Module TM3.
+Definition tm := Eval compute in (TM_from_str "1RB0RC---_2RC0LB1LB_2LC2RA2RB").
+Notation "c -->* c'" := (c -[ tm ]->* c') (at level 40).
+Notation "c -->+ c'" := (c -[ tm ]->+ c') (at level 40).
+
+Notation h0 := ((C,<[]),(B,[])).
+Notation h1 := ((A,<[2]),(B,[])).
+Notation h2 := ((B,<[2;1]),(B,[])).
+
+Definition f1 (w:seg)(h:head):option((list seg)*(list head)) :=
+List.find (fun '(x,y) => eqb x (h,w)) (
+((h0,[1;1]),([[1;1]],[h0;h0]))::
+((h0,[1;0;1]),([[1;0;0]],[]))::
+((h0,[1;0;0]),([[1;0;1]],[h0]))::
+((h1,[1;1]),([[1;1]],[h1;h0]))::
+((h1,[1;0;1]),([[1;1];[2;1]],[]))::
+((h0,[2;1]),([[1;0]],[]))::
+((h0,[1;0]),([],[h2]))::
+((h2,[1;0;1]),([[1;0;0;0;1]],[]))::
+((h0,[1;0;0;0;1]),([[1;0;1];[1;1]],[]))::
+((h2,[1;0;0]),([[1;0;0;0;0]],[]))::
+((h0,[1;0;0;0;0]),([[1;0;1];[1;0]],[]))::
+((h0,[2;0]),([[1;1]],[h0]))::
+((h1,[1;0;0]),([[1;1];[2;0]],[]))::
+((h2,[1;1]),([[1;0;0];[1]],[]))::
+((h0,[1]),([],[h1]))::
+nil) &&& (fun '(x,y) => Some y).
+
+Definition f0 (w:seg)(h:head):option((list seg)*seg) :=
+List.find (fun '(x,y) => eqb x (h,w)) (
+((h0,[1]),([[1;0;1]],[1]))::
+nil) &&& (fun '(x,y) => Some y).
+
+Definition f2 (w:seg)(h:head):option(N*N*head) :=
+List.find (fun '(x,y) => eqb x (h,w)) (
+((h0,[1;1]),(0%N,1%N,h0))::
+((h0,[1;0;1]),(1%N,0%N,h0))::
+((h0,[1;0;0]),(1%N,0%N,h0))::
+nil) &&& (fun '(x,y) => Some y).
+
+Definition ws_init:(list seg)*seg := ([[1;1];[1;1];[1;1];[1;1];[1;1];[1;0;1];[1;0;1];[1;0;0];[1;0;0]],[1]).
+
+Definition hs_step:(list head) := [h1]^^30.
+
+
+Lemma nonhalt: ~halts tm c0.
+Proof.
+  eapply decide_nonhalt_spec with
+  (tm:=tm) (f2:=f2) (f1:=f1) (f0:=f0) (hs_step:=hs_step) (ws_init:=ws_init)
+  (lh:=0inf<*<[2]) (pp:=1%nat) (T:=N.to_nat (10^5)).
+  - intros.
+    unfold f2 in H.
+    apply find_spec in H.
+    gen w h a0 a1 h'.
+    apply f2_spec' with (T:=(10^3)).
+    time vm_compute; reflexivity.
+  - intros.
+    unfold f1 in H.
+    apply find_spec in H.
+    gen w h ws hs.
+    apply f1_spec' with (T:=(10^3)).
+    match goal with
+    | |- List.forallb ?f ?x = _ =>
+      pose (List.map f x) as v1;
+      vm_compute in v1
+    end.
+    time vm_compute; reflexivity.
+  - intros.
+    unfold f0 in H.
+    apply find_spec in H.
+    gen w h w'.
+    apply f0_spec' with (T:=(10^3)).
+    time vm_compute; reflexivity.
+  - reflexivity.
+  - intro X; inverts X.
+  - apply BoundedConfig.sideRLs_c_spec with (T:=10^4); reflexivity.
+  - stepn 484%N.
+  - native_check_eq.
+Time Qed.
+
+End TM3.
+
+
+Module TM4.
+Definition tm := Eval compute in (TM_from_str "1LB2RB0RC_2RA2LA1LB_---2RA1RC").
+Notation "c -->* c'" := (c -[ tm ]->* c') (at level 40).
+Notation "c -->+ c'" := (c -[ tm ]->+ c') (at level 40).
+
+Notation h0 := ((C,<[]),(B,[])).
+Notation h1 := ((A,<[2]),(B,[])).
+Notation h2 := ((C,<[0]),(B,[])).
+
+Definition f1 (w:seg)(h:head):option((list seg)*(list head)) :=
+List.find (fun '(x,y) => eqb x (h,w)) (
+((h0,[1;1;1;2]),([[1;1;1;2]],[h0;h0]))::
+((h0,[1;1;2]),([[1;1;1]],[]))::
+((h0,[1;1;1]),([[1;1;2]],[h0]))::
+((h1,[1;1;1;2]),([[1;1;2];[1]],[h2]))::
+((h2,[1;1;1;2]),([[1;1;2;1]],[h0;h0;h2]))::
+((h2,[1;1;1]),([[1;1;1;2]],[h0;h0;h0]))::
+((h0,[1]),([],[h1]))::
+((h1,[1;1;2;1]),([[1;1;1;2]],[h1;h0]))::
+((h2,[1;1;2]),([[1;1;2]],[h1]))::
+((h1,[1;1;2]),([[1;1;1;2]],[h0;h0]))::
+((h1,[1;1;1]),([[1;1;2]],[h1]))::
+nil) &&& (fun '(x,y) => Some y).
+
+Definition f0 (w:seg)(h:head):option((list seg)*seg) :=
+List.find (fun '(x,y) => eqb x (h,w)) (
+((h0,[1;1]),([[1;1;1]],[1]))::
+((h0,[1]),([],[1;1]))::
+nil) &&& (fun '(x,y) => Some y).
+
+Definition f2 (w:seg)(h:head):option(N*N*head) :=
+List.find (fun '(x,y) => eqb x (h,w)) (
+((h0,[1;1;1;2]),(0%N,1%N,h0))::
+((h0,[1;1;2]),(1%N,0%N,h0))::
+((h0,[1;1;1]),(1%N,0%N,h0))::
+((h2,[1;1;2]),(0%N,0%N,h1))::
+nil) &&& (fun '(x,y) => Some y).
+
+Definition ws_init:(list seg)*seg := ([[1;1;1;2];[1;1;1;2];[1;1;1;2];[1;1;1];[1;1;1;2];[1;1;1;2];[1;1;1];[1;1;1;2];[1;1;2];[1;1;1];[1;1;2];[1;1;2];[1;1;2]],[1;1]).
+
+Definition hs_step:(list head) := [h1;h0;h2]^^65.
+
+Lemma nonhalt: ~halts tm c0.
+Proof.
+  eapply decide_nonhalt_spec with
+  (tm:=tm) (f2:=f2) (f1:=f1) (f0:=f0) (hs_step:=hs_step) (ws_init:=ws_init)
+  (lh:=0inf<*<[2;0;1;1]) (pp:=2%nat) (T:=N.to_nat (10^5)).
+  - intros.
+    unfold f2 in H.
+    apply find_spec in H.
+    gen w h a0 a1 h'.
+    apply f2_spec' with (T:=(10^3)).
+    time vm_compute; reflexivity.
+  - intros.
+    unfold f1 in H.
+    apply find_spec in H.
+    gen w h ws hs.
+    apply f1_spec' with (T:=(10^3)).
+    time vm_compute; reflexivity.
+  - intros.
+    unfold f0 in H.
+    apply find_spec in H.
+    gen w h w'.
+    apply f0_spec' with (T:=(10^3)).
+    time vm_compute; reflexivity.
+  - reflexivity.
+  - intro X; inverts X.
+  - apply BoundedConfig.sideRLs_c_spec with (T:=10^4); reflexivity.
+  - stepn 3462%N.
+  - native_check_eq.
+Time Qed.
+
+End TM4.
+
